Makefile
@@ -2,7 +2,7 @@ DFY_FILES := $(shell find src -name "*.dfy")
 OK_FILES := $(DFY_FILES:.dfy=.dfy.ok)
 
 # these arguments don't affect verification outcomes
-DAFNY_BASIC_ARGS := /compile:0 /compileTarget:go /timeLimit:40 /vcsLoad:0.5
+DAFNY_BASIC_ARGS := /compile:0 /compileTarget:go /timeLimit:30 /vcsLoad:0.5
 DAFNY_ARGS := /noNLarith /arith:5
 DAFNY=./etc/dafnyq $(DAFNY_BASIC_ARGS) $(DAFNY_ARGS)
 
